---
layout: post
section-type: post
title: Math Cheat Sheet
category: Keypoint
tags: [ 'reading' ]
comments: true
---
<head>
<script src='https://cdnjs.cloudflare.com/ajax/libs/mathjax/2.7.5/latest.js?config=TeX-MML-AM_CHTML' async></script>
<script type="text/javascript" src="http://www.hostmath.com/Math/MathJax.js?config=OK"></script>
</head>


### Logarithm Rules
<br>
> \begin{equation}log_{b}(M\;\*\;N)\;=\;log_{b}M\;+\;log_{b}N\end{equation}
> \begin{equation}log_{b}(\frac{M}{N})\;=\;log_{b}M\;-\;log_{b}N\end{equation}
> \begin{equation}log_{b}(M^{k})\;=\;k\;*\;log_{b}M\end{equation}
> \begin{equation}log_{b}(1)\;=\;0\end{equation}
> \begin{equation}log_{b}(b)\;=\;1\end{equation}
> \begin{equation}log_{b}(b^{k})\;=\;k\end{equation}
> \begin{equation}b^{log_{b}(k)}\;=\;k\end{equation}
> \begin{equation}log_{b}(M)\;=\;\frac{ln(M)}{ln(b)}\end{equation}
> Where: _b > 1_, and _M_, _N_ and _k_ can be any **real numbers**, but _M_ & _N_ MUST be **positive**!

<br>
<hr>
<br>

### Derivative Rules
> \begin{equation}\frac{\partial}{\partial x}(log_{b}(u(x)))\;=\;ln(b)\*\frac{\partial u(x)}{\partial x}\end{equation}
> \begin{equation}\frac{\partial}{\partial x}b^{u(x)}\;=\;ln(b)\*b^{u(x)}\*\frac{\partial u(x)}{\partial x}\end{equation}
> \begin{equation}\frac{\partial}{\partial x}c\*u(x)\;=\;c\*\frac{\partial u(x)}{\partial x}\end{equation}
> \begin{equation}\frac{\partial}{\partial x}u(x)\;+\;v(x)\;=\frac{\partial u(x)}{\partial x}\;+\;\frac{\partial v(x)}{\partial x}\end{equation}
> \begin{equation}\frac{\partial}{\partial x}u(x)\;-\;v(x)\;=\frac{\partial u(x)}{\partial x}\;-\;\frac{\partial v(x)}{\partial x}\end{equation}
> \begin{equation}\frac{\partial}{\partial x}u(x)\*v(x)\;=\;u(x)\*\frac{\partial v(x)}{\partial x}\;+\;v(x)\*\frac{\partial u(x)}{\partial x}\end{equation}
> \begin{equation}\frac{\partial}{\partial x}\frac{u(x)}{v(x)}\;=\;(v(x)\*\frac{\partial u(x)}{\partial x}\;-\;u(x)\*\frac{\partial v(x)}{\partial x})\*(v(x))^{-2}\end{equation}
> \begin{equation}\frac{\partial}{\partial x}\frac{1}{u(x)}\;=\;-\frac{\partial u(x)}{\partial x}\*(u(x))^{-2}\end{equation}
> \begin{equation}\frac{\partial y}{\partial x}\;=\;\frac{\partial y}{\partial u}\*\frac{\partial u}{\partial x}\end{equation}

<br>
<hr>
<br>

> #### Integration Rules
> \begin{equation}\int u\frac{\partial v}{\partial x}\partial x\;=\;uv\;-\;\int v\frac{\partial u}{\partial x}\partial x\end{equation}
> Note: from _u_, get _du/dx_, from _dv/dx_, get _v_, then assemble the right side of the rule.
> \begin{equation}\int c\*u(x)\partial x\;=\;c\int u(x)\partial x\end{equation}
> \begin{equation}\int (u(x)\;+\;v(x))\partial x\;=\;\int u(x)\partial x\;+\;\int v(x)\partial x\end{equation}
> \begin{equation}\int (u(x)\;-\;v(x))\partial x\;=\;\int u(x)\partial x\;-\;\int v(x)\partial x\end{equation}
> \begin{equation}\int b^{x}\partial x\;=\;\frac{b^{x}}{ln(b)}\;+\;C\end{equation}

<br>
<hr>
<br>

> \begin{equation}\end{equation}
> \begin{equation}\end{equation}
> \begin{equation}\end{equation}
> \begin{equation}\end{equation}


<br>

<hr>

#### Resources:

<br>
